sir/Sir/Spec/Run.lean
@@ -16,13 +16,4 @@ def Program.RunsTo (program : Program) (ctx : CallContext) (entry : FunctionId)
     (world : World) (trace : Trace) (final : MachineState) : Prop :=
   program.Runs ctx entry world trace final ∧ final.control = .halted
 
-def Program.RunsInit (program : Program) (ctx : CallContext)
-    (world : World) (trace : Trace) (final : Globals) : Prop :=
-  EvalFn program ctx program.initEntry { world := world } #[] trace final .halted
-
-def Program.RunsMain (program : Program) (ctx : CallContext)
-    (world : World) (trace : Trace) (final : Globals) : Prop :=
-  ∃ entry, program.mainEntry = some entry ∧
-    EvalFn program ctx entry { world := world } #[] trace final .halted
-
 end Sir
